aps_plus/ -> aps_plus_2/.

theories/aps_plus_2/examples/list_length.v
@@ -6,67 +6,67 @@ From simuliris.data_human_lang Require Export
   compilation.
 From simuliris.data_human_lang Require Import
   notations.
-From simuliris.aps_plus Require Import
+From simuliris.aps_plus_2 Require Import
   definition.
 
-Definition list_sum : data_human_program := {[
-  "list_sum" := (BNamed "arg", (
+Definition list_length : data_human_program := {[
+  "list_length" := (BNamed "arg", (
     match: ![𝟙] "arg" with
       NIL =>
         0
-    | CONS "x", "xs" =>
-        "x" + $"list_sum" "xs"
+    | CONS <>, "xs" =>
+        1 + $"list_length" "xs"
     end
   )%data_human_expr)
 ]}.
 
-Definition list_sum_aps_plus : data_human_program := {[
-  "list_sum" := (BNamed "arg", (
+Definition list_length_aps_plus : data_human_program := {[
+  "list_length" := (BNamed "arg", (
     match: ![𝟙] "arg" with
       NIL =>
         0
-    | CONS "x", "xs" =>
-        let: "acc" := "x" in
+    | CONS "<>", "xs" =>
+        let: "acc" := 1 in
         let: "arg" := "xs" in
-        $"list_sum_aps" ("acc", "arg")
+        $"list_length_aps" ("acc", "arg")
     end
   )%data_human_expr) ;
-  "list_sum_aps" := (BNamed "arg", (
+  "list_length_aps" := (BNamed "arg", (
     let: "acc" := ![𝟙] "arg" in
     let: "arg" := ![𝟚] "arg" in
     match: ![𝟙] "arg" with
       NIL =>
         0 + "acc"
-    | CONS "x", "xs" =>
-        let: "acc" := "x" + "acc" in
+    | CONS "<>", "xs" =>
+        let: "acc" := 1 + "acc" in
         let: "arg" := "xs" in
-        $"list_sum_aps" ("acc", "arg")
+        $"list_length_aps" ("acc", "arg")
     end
   )%data_human_expr)
 ]}.
 
-Section list_sum_aps_plus_sound.
+Section list_length_aps_plus_sound.
   Variable aps_plus_sound : ∀ progₛ progₜ,
     data_program_valid progₛ →
     aps_plus progₛ progₜ →
     data_program_refinement progₛ progₜ.
 
-  Lemma list_sum_aps_plus_sound :
+  Lemma list_length_aps_plus_sound :
     data_program_refinement
-      (data_human_program_compile list_sum)
-      (data_human_program_compile list_sum_aps_plus).
+      (data_human_program_compile list_length)
+      (data_human_program_compile list_length_aps_plus).
   Proof using aps_plus_sound.
-    rewrite /list_sum /list_sum_aps_plus. apply aps_plus_sound.
+    rewrite /list_length /list_length_aps_plus. apply aps_plus_sound.
     - split.
       + apply data_human_program_compile_well_formed.
         rewrite /data_human_program_well_formed map_Forall_singleton //.
       + apply data_human_program_compile_scope.
     - rewrite /data_human_program_compile map_fmap_singleton fmap_insert map_fmap_singleton /=.
-      exists {["list_sum" := "list_sum_aps"]}; try set_solver.
+      exists {["list_length" := "list_length_aps"]}; try set_solver.
       + intros * (<- & <-)%lookup_singleton_Some.
         rewrite lookup_insert.
         eexists. split; last done. repeat econstructor.
       + intros * (<- & <-)%lookup_singleton_Some (_ & <-)%lookup_singleton_Some.
         eexists. split; last done. repeat econstructor.
   Qed.
-End list_sum_aps_plus_sound.
+End list_length_aps_plus_sound.
